

1. split the sum

$$= \frac{1}{N} \left(\sum_{i=1}^n a + \sum_{i=1}^N b x_i \right)$$

since a/b constants

$$= \frac{1}{N} \left(Na + b \sum_{i=1}^N x_i \right)$$

$$= a + b \left(\frac{1}{N} \sum_{i=1}^N x_i \right)$$

$$= a + b m(X)$$

2.

$$\text{cov}(X, X) = \frac{1}{N} \sum_{i=1}^N (x_i - m(X))(x_i - m(X))$$

$$= \frac{1}{N} \sum_{i=1}^N (x_i - m(X))^2$$

def of sample var

$$s^2 = \frac{1}{N} \sum_{i=1}^N (x_i - m(X))^2$$

$$\text{Therefore } (X, X) = s^2$$

3,

$$\text{cov}(X, a+bY) = \frac{1}{N} \sum_{i=1}^N (x_i - m(X)) [(a+by_i) - m(a+bY)]$$

part (1)

$$m(a+bY) = a + bm(Y)$$

inside sum

$$(a+by_i) - (a+bm(Y)) = b(y_i - m(Y))$$

Thus:

$$= \frac{1}{N} \sum_{i=1}^N (x_i - m(X)) \cdot b(y_i - m(Y))$$

Factor out b .

$$= b \cdot \frac{1}{N} \sum_{i=1}^N (x_i - m(X)) (y_i - m(Y))$$

$$= b \text{cov}(X, Y)$$

4. Show that

apply part 3 twice

$$\text{cov}(a+bX, a+bY) = b \text{cov}(X, a+bY)$$

from part (3)

$$\text{cov}(X, a+bY) = b \text{cov}(X, Y)$$

So:

$$b \cdot b \cdot \text{cov}(X, Y) = b^2 \text{cov}(X, Y)$$

Showing

$$\text{cov}(bX$$

5.

$$\text{Let } \text{IQR}(X) = Q_3(X) - Q_1(X)$$

Then

$$Q_3(a+bX) = a + bQ_3(X), \quad Q_1(a+bX) = a + bQ_1(X)$$

So

$$\text{IQR}(a+bX) = b(Q_3(X) - Q_1(X)) = b \text{IQR}(X)$$

$$\text{So additive cancels out } a + b \text{IQR}(X)$$

6. Let $X = \{1, 4\}$

Simple example $m(X) = \frac{1+4}{2} = 2.5$

$$(m(X))^2 = 6.25$$

Now compute

$$X^2 = \{1, 16\} \Rightarrow m(X^2) = \frac{1+16}{2} = 8.5$$

$$m(X^2) \neq (m(X))^2$$